coq/cclc/clc_validity.v
@@ -40,57 +40,45 @@ Proof with eauto using ok.
     split... }
 Qed.
 
-Theorem validity Γ m A :
-  ok Γ -> Γ ⊢ m : A -> exists s l, [Γ] ⊢ A : s @ l.
+Theorem validity Γ m A s :
+  ok Γ -> Γ ⊢ m : A : s -> exists l, [Γ] ⊢ A : s @ l : U.
 Proof with eauto using clc_type, re_pure, merge_re_id.
-  move=>wf tp. elim: tp wf=>{Γ m A}.
-  move=>Γ s l k o.
-    exists U. exists l.+2...
-  move=>Γ A B s r t i k tyA ihA tyB ihB o.
-    exists U. exists i.+1...
-  move=>Γ x A s hs o.
-    move:(has_ok o hs)=>[l tyA].
-    exists s. exists l...
-  move=>Γ A B m s t i k tyP ihP tym ihm o.
-    exists t. exists i...
-  move=>Γ1 Γ2 Γ A B m n s t k mrg tym ihm tyn ihn o.
+  move=>wf tp. elim: tp wf=>{Γ m A s}.
+  move=>Γ s l k o. exists l.+2...
+  move=>Γ A B s r t i k tyA ihA tyB ihB o. exists i.+1...
+  move=>Γ x A s hs o. move:(has_ok o hs)=>[l tyA]. exists l...
+  move=>Γ A B m s r t i k tyP ihP tym ihm o. exists i...
+  move=>Γ1 Γ2 Γ A B m n s r t k mrg tym ihm tyn ihn o.
     move:(merge_context_ok_inv mrg o)=>[o1 o2].
     move:(merge_re_re mrg)=>[e1[e2 e3]].
-    move:o1=>/ihm{ihm}[r1[l1 /pi_inv[r2[l2[tyA tyB]]]]].
-    destruct s.
-    exists r2. exists l2.
+    move:o1=>/ihm{ihm}[l1/pi_inv[l2[tyA[_ tyB]]]].
+    destruct s; exists l2.
     have {}mrg : [Γ1] ∘ Γ2 => [Γ].
       replace Γ2 with [Γ2].
       rewrite e2 e3...
       rewrite<-pure_re...
     by apply: (substitution tyB k mrg tyn).
-    exists r2. exists l2.
     move:(substitutionN tyB tyn).
     by rewrite e2.
-  move=>Γ k o. exists U. exists 1...
-  move=>Γ k o. exists U. exists 0...
-  move=>Γ A B s r t i leq k tyA ihA tyB ihB o.
-    exists U. exists i.+1...
+  move=>Γ k o. exists 1...
+  move=>Γ k o. exists 0...
+  move=>Γ A B s r t i leq k tyA ihA tyB ihB o. exists i.+1...
   move=>Γ1 Γ2 Γ A B m n s r t i k1 k2 mrg
-    tyS ihS tym ihm tyn ihn o.
-    exists t. exists i...
-  move=>Γ1 Γ2 Γ m n A mrg _ _ tyn ihn o.
-    move:(merge_context_ok_inv mrg o)=>[_/ihn[x[l tyA]]]{ihn}.
+    tyS ihS tym ihm tyn ihn o. exists i...
+  move=>Γ1 Γ2 Γ m n A s mrg _ _ tyn ihn o.
+    move:(merge_context_ok_inv mrg o)=>[_/ihn[l tyA]]{ihn}.
     move:(merge_re_re mrg)=>[_[_ e]].
-    exists x. exists l.
-    by rewrite<-e.
+    exists l. by rewrite<-e.
   move=>Γ1 Γ2 Γ A B C m n s r t k x i leq key mrg
-    tym _ tyC _ tyn _ o.
-    exists x. exists i.
+    tym _ tyC _ tyn _ o. exists i.
     move:(merge_re_re mrg)=>[e0[e1 e2]].
     destruct k; simpl in tyC.
     have mrg1:[Γ2] ∘ Γ1 => [Γ].
     rewrite e2 (pure_re key) e1.
-    apply: merge_re_id.
+    apply: merge_re_id. inv leq.
     have:=substitution tyC key mrg1 tym.
     by asimpl.
     have:=substitutionN tyC tym.
     by rewrite e2.
-  move=>Γ A B m s i sb tym ihm tyB ihB o.
-    exists s. exists i...
+  move=>Γ A B m s i sb tym ihm tyB ihB o. exists i...
 Qed.
